src/Context.v
@@ -1,0 +1,81 @@
+Require Import LinearScan.Lib.
+
+Set Implicit Arguments.
+Unset Strict Implicit.
+Unset Printing Implicit Defensive.
+Generalizable All Variables.
+
+Section Context.
+
+Variable errType : Set.
+
+(* The Indexed Reader State Either monad. *)
+Definition Context (i o a : Type) := seq errType -> i -> seq errType + (a * o).
+
+Definition iask {i} : Context i i (seq errType) := fun e i => inr (e, i).
+Definition iget {i} : Context i i i := fun _ i => inr (i, i).
+Definition iput {i o} (x : o) : Context i o unit := fun _ _ => inr (tt, x).
+
+Definition imap {I O X Y} : (X -> Y) -> Context I O X -> Context I O Y :=
+  fun f x e st =>
+    match x e st with
+    | inl err     => inl err
+    | inr (a,st') => inr (f a, st')
+    end.
+
+Definition ipure {I X} : X -> Context I I X := fun x _ st => inr (x, st).
+
+Definition ijoin {I A O X} : Context I A (Context A O X) -> Context I O X :=
+  fun x e st =>
+    match x e st with
+    | inl err => inl err
+    | inr (y, st') =>
+        match y e st' with
+        | inl err => inl err
+        | inr (a, st'') => inr (a, st'')
+        end
+    end.
+
+Definition ibind {I A O X Y} (f : X -> Context A O Y) (x : Context I A X) :
+  Context I O Y := @ijoin I A O Y (@imap I A X _ f x).
+
+Definition conseq `(x : Context P2 Q2 a) `(f : P1 -> P2) `(g : Q2 -> Q1) :
+  Context P1 Q1 a.
+Proof.
+  rewrite /Context in x *.
+  move=> e p.
+  case (x e (f p)) => [e'|[a' q]].
+    exact: inl e'.
+  apply: inr (a', _).
+  exact: g q.
+Defined.
+
+Definition strengthen `(x : Context P2 Q a) `(f : P1 -> P2) : Context P1 Q a :=
+  conseq x f id.
+
+Definition weaken `(x : Context P Q2 a) `(g : Q2 -> Q1) : Context P Q1 a :=
+  conseq x id g.
+
+End Context.
+
+Set Maximal Implicit Insertion.
+
+Arguments iask : default implicits.
+Arguments iget : default implicits.
+Arguments iput : default implicits.
+Arguments imap : default implicits.
+Arguments ipure : default implicits.
+Arguments ijoin : default implicits.
+Arguments ibind : default implicits.
+Arguments conseq : default implicits.
+Arguments strengthen : default implicits.
+Arguments weaken : default implicits.
+
+Unset Maximal Implicit Insertion.
+
+Notation "m >>>= f" := (ibind f m) (at level 25, left associativity).
+
+Notation "X <<- A ;;; B" := (A >>>= (fun X => B))
+  (at level 92, A at next level, right associativity).
+
+Notation "A ;;; B" := (_ <<- A ;;; B) (at level 92, right associativity).
